spec/design/skel/PSpaceStorable_H.thy
@@ -27,6 +27,7 @@ datatype
   | CTET
   | TCBT
   | UserDataT
+  | UserDataDeviceT
   | KernelDataT
   | ArchT arch_kernel_object_type
 
@@ -38,6 +39,7 @@ where
 | "koTypeOf (KOCTE e) = CTET"
 | "koTypeOf (KOTCB e) = TCBT"
 | "koTypeOf (KOUserData) = UserDataT"
+| "koTypeOf (KOUserDataDevice) = UserDataDeviceT"
 | "koTypeOf (KOKernelData) = KernelDataT"
 | "koTypeOf (KOArch e) = ArchT (archTypeOf e)"
 
